@prefix : <http://www.semanticweb.org/italian-research-organization#> .
@prefix owl: <http://www.w3.org/2002/07/owl#> .
@prefix rdf: <http://www.w3.org/1999/02/22-rdf-syntax-ns#> .
@prefix xml: <http://www.w3.org/XML/1998/namespace> .
@prefix xsd: <http://www.w3.org/2001/XMLSchema#> .
@prefix rdfs: <http://www.w3.org/2000/01/rdf-schema#> .
@prefix dctypes: <http://purl.org/dc/dcmitype/> .
@base <http://www.semanticweb.org/italian-research-organization> .

<http://www.semanticweb.org/italian-research-organization> rdf:type owl:Ontology .

#################################################################
#    Object Properties
#################################################################

###  http://www.semanticweb.org/italian-research-organization#hasBuilding
:hasBuilding rdf:type owl:ObjectProperty ;
             rdfs:subPropertyOf :hasPart ;
             owl:inverseOf :isBuildingOf ;
             rdf:type owl:InverseFunctionalProperty ;
             rdfs:domain :Institute ;
             rdfs:range :Building ;
             rdfs:comment "hasBuilding is a subproperty of hasPart and relates an institute to buildings that belongs to it."@en ;
             rdfs:label "has building"@en .


###  http://www.semanticweb.org/italian-research-organization#hasContractWith
:hasContractWith rdf:type owl:ObjectProperty ;
                 owl:inverseOf :makesContractWith ;
                 rdf:type owl:FunctionalProperty ;
                 rdfs:domain :Employee ;
                 rdfs:range :ResearchOrganisation ;
                 rdfs:comment "hasContractWith relates an employee to the research organization with which he has a contract."@en ;
                 rdfs:label "has a contract with"@en .


###  http://www.semanticweb.org/italian-research-organization#hasInstitute
:hasInstitute rdf:type owl:ObjectProperty ;
              rdfs:subPropertyOf :hasPart ;
              owl:inverseOf :isInstituteOf ;
              rdf:type owl:InverseFunctionalProperty ;
              rdfs:domain :ResearchOrganisation ;
              rdfs:range :Institute ;
              rdfs:comment "hasInstitute is a subproperty of hasPart and relates a research organization to institutes that compose it"@en ;
              rdfs:label "has institute"@en .


###  http://www.semanticweb.org/italian-research-organization#hasInstituteMember
:hasInstituteMember rdf:type owl:ObjectProperty ;
                    rdfs:subPropertyOf :hasMember ;
                    owl:inverseOf :isMemberOfInstitute ;
                    rdf:type owl:InverseFunctionalProperty ;
                    rdfs:domain :Institute ;
                    rdfs:range :Employee ;
                    rdfs:comment "hasInstituteMember relates an institute to its members, that are empoyees"@en ;
                    rdfs:label "has institute member"@en .


###  http://www.semanticweb.org/italian-research-organization#hasLaboratory
:hasLaboratory rdf:type owl:ObjectProperty ;
               rdfs:subPropertyOf :hasPart ;
               owl:inverseOf :isLaboratoryOf ;
               rdf:type owl:InverseFunctionalProperty ;
               rdfs:domain :Institute ;
               rdfs:range :Laboratory ;
               rdfs:comment "hasLaboratory is a subproperty of hasPart and relates an institute to laboratories that compose it"@en ;
               rdfs:label "has laboratory"@en .


###  http://www.semanticweb.org/italian-research-organization#hasLaboratoryMember
:hasLaboratoryMember rdf:type owl:ObjectProperty ;
                     rdfs:subPropertyOf :hasMember ;
                     owl:inverseOf :isMemberOfLaboratory ;
                     rdf:type owl:InverseFunctionalProperty ;
                     rdfs:domain :Laboratory ;
                     rdfs:range [ rdf:type owl:Class ;
                                  owl:unionOf ( :Researcher
                                                :Technologist
                                              )
                                ] ;
                     rdfs:comment "hasLaboratoryMember relates a Laboratory with its members. Each member is a Researchers or a Technologist."@en ;
                     rdfs:label "has laboratory member"@en .


###  http://www.semanticweb.org/italian-research-organization#hasLocation
:hasLocation rdf:type owl:ObjectProperty ;
             owl:inverseOf :isLocationOf ;
             rdf:type owl:FunctionalProperty ;
             rdfs:domain :Building ;
             rdfs:range :Location ;
             rdfs:comment "hasLocation relates a building to the location where it is placed"@en ;
             rdfs:label "has location"@en .


###  http://www.semanticweb.org/italian-research-organization#hasMeetingRoom
:hasMeetingRoom rdf:type owl:ObjectProperty ;
                rdfs:subPropertyOf :hasPart ;
                owl:inverseOf :isMeetingRoomOf ;
                rdf:type owl:InverseFunctionalProperty ;
                rdfs:domain :Building ;
                rdfs:range :MeetingRoom ;
                rdfs:comment "hasMeetingRoom is a subproperty of hasPart and relates a meeting room to the building it belongs to"@en ;
                rdfs:label "has meeting room"@en .


###  http://www.semanticweb.org/italian-research-organization#hasMember
:hasMember rdf:type owl:ObjectProperty ;
           owl:inverseOf :isMemberOf ;
           rdf:type owl:ReflexiveProperty ;
           rdfs:comment "hasMember is superproperty of: hasInstituteMember, hasResearchGroupMember, hasLaboratoryMember"@en ;
           rdfs:label "has member"@en .


###  http://www.semanticweb.org/italian-research-organization#hasOffice
:hasOffice rdf:type owl:ObjectProperty ;
           rdfs:subPropertyOf :hasPart ;
           owl:inverseOf :isOfficeOf ;
           rdf:type owl:InverseFunctionalProperty ;
           rdfs:domain :Building ;
           rdfs:range :Office ;
           rdfs:comment "hasOffice is a subproperty of hasPart and relates a building to the offices belonging to it"@en ;
           rdfs:label "has office"@en .


###  http://www.semanticweb.org/italian-research-organization#hasPart
:hasPart rdf:type owl:ObjectProperty ;
         owl:inverseOf :isPartOf ;
         rdf:type owl:TransitiveProperty ,
                  owl:ReflexiveProperty ;
         rdfs:comment "hasPart is a superproperty of: hasInstitute, hasLaboratory, hasResearchGroup, hasBuilding, has Office and hasMeetingRoom"@en ;
         rdfs:label "has part"@en .


###  http://www.semanticweb.org/italian-research-organization#hasResearchGroup
:hasResearchGroup rdf:type owl:ObjectProperty ;
                  rdfs:subPropertyOf :hasPart ;
                  owl:inverseOf :isResearchGroupOf ;
                  rdf:type owl:InverseFunctionalProperty ;
                  rdfs:domain :Laboratory ;
                  rdfs:range :ResearchGroup ;
                  rdfs:comment "hasResearchGroup is a subproperty of hasPart and relates laboratory with research groups that compose it"@en ;
                  rdfs:label "has research group"@en .


###  http://www.semanticweb.org/italian-research-organization#hasResearchGroupMember
:hasResearchGroupMember rdf:type owl:ObjectProperty ;
                        rdfs:subPropertyOf :hasMember ;
                        owl:inverseOf :isMemberOfResearchGroup ;
                        rdf:type owl:InverseFunctionalProperty ;
                        rdfs:domain :ResearchGroup ;
                        rdfs:range [ rdf:type owl:Class ;
                                     owl:unionOf ( :Researcher
                                                   :Technologist
                                                 )
                                   ] ;
                        rdfs:comment "hasResearchGroupMember relates a ResearchGroup with its members. Each member is a Researcher or a Technologist."@en ;
                        rdfs:label "has research group member"@en .


###  http://www.semanticweb.org/italian-research-organization#hosts
:hosts rdf:type owl:ObjectProperty ;
       owl:inverseOf :isHostedIn ;
       rdf:type owl:InverseFunctionalProperty ;
       rdfs:domain :Office ;
       rdfs:range :Employee ;
       rdfs:comment "hosts relates an office to employees that work in it"@en ;
       rdfs:label "hosts"@en .


###  http://www.semanticweb.org/italian-research-organization#isBuildingOf
:isBuildingOf rdf:type owl:ObjectProperty ;
              rdfs:subPropertyOf :isPartOf ;
              rdf:type owl:FunctionalProperty ;
              rdfs:domain :Building ;
              rdfs:range :Institute ;
              rdfs:comment "isBuildingOf is a subproperty of isPartOf and relates buildings to the institute they belong to"@en ;
              rdfs:label "is building of"@en .


###  http://www.semanticweb.org/italian-research-organization#isHostedIn
:isHostedIn rdf:type owl:ObjectProperty ,
                     owl:FunctionalProperty ;
            rdfs:domain :Employee ;
            rdfs:range :Office ;
            rdfs:comment "isHostedIn relates employees to the office in which they works"@en ;
            rdfs:label "is hosted in"@en .


###  http://www.semanticweb.org/italian-research-organization#isInstituteOf
:isInstituteOf rdf:type owl:ObjectProperty ;
               rdfs:subPropertyOf :isPartOf ;
               rdf:type owl:FunctionalProperty ;
               rdfs:domain :Institute ;
               rdfs:range :ResearchOrganisation ;
               rdfs:comment "isIntituteOf is a subproperty of isPartOf and relates intitutes to the research organization of which it is composed"@en ;
               rdfs:label "is institute of"@en .


###  http://www.semanticweb.org/italian-research-organization#isLaboratoryOf
:isLaboratoryOf rdf:type owl:ObjectProperty ;
                rdfs:subPropertyOf :isPartOf ;
                rdf:type owl:FunctionalProperty ;
                rdfs:domain :Laboratory ;
                rdfs:range :Institute ;
                rdfs:comment "isLaboratoryOf is a subproperty of isPartOf and relates laboratories to the institute of which it is composed"@en ;
                rdfs:label "is laboratory of"@en .


###  http://www.semanticweb.org/italian-research-organization#isLocationOf
:isLocationOf rdf:type owl:ObjectProperty ,
                       owl:InverseFunctionalProperty ;
              rdfs:domain :Location ;
              rdfs:range :Building ;
              rdfs:comment "isLocationOf relates a location to buildings that are placed there"@en ;
              rdfs:label "is location of"@en .


###  http://www.semanticweb.org/italian-research-organization#isMeetingRoomOf
:isMeetingRoomOf rdf:type owl:ObjectProperty ;
                 rdfs:subPropertyOf :isPartOf ;
                 rdf:type owl:FunctionalProperty ;
                 rdfs:domain :MeetingRoom ;
                 rdfs:range :Building ;
                 rdfs:comment "isMeetingRoomOf is a subproperty of isPartOf and relates a meeting room to the building it belongs to"@en ;
                 rdfs:label "is meeting room of"@en .


###  http://www.semanticweb.org/italian-research-organization#isMemberOf
:isMemberOf rdf:type owl:ObjectProperty ,
                     owl:ReflexiveProperty ;
            rdfs:comment "isMemberOf is a superproperty of: isMemberOfInstitute, isMemberOfLaboratory and isMemberOfResearchGroup"@en ;
            rdfs:label "is member of"@en .


###  http://www.semanticweb.org/italian-research-organization#isMemberOfInstitute
:isMemberOfInstitute rdf:type owl:ObjectProperty ;
                     rdfs:subPropertyOf :isMemberOf ;
                     rdf:type owl:FunctionalProperty ;
                     rdfs:domain :Employee ;
                     rdfs:range :Institute ;
                     rdfs:comment "isMemberOfInstitute is a subproperty of isMemberOf and relates an employee to the institute of which he is a member"@en ;
                     rdfs:label "is member of institute"@en .


###  http://www.semanticweb.org/italian-research-organization#isMemberOfLaboratory
:isMemberOfLaboratory rdf:type owl:ObjectProperty ;
                      rdfs:subPropertyOf :isMemberOf ;
                      rdf:type owl:FunctionalProperty ;
                      rdfs:domain [ rdf:type owl:Class ;
                                    owl:unionOf ( :Researcher
                                                  :Technologist
                                                )
                                  ] ;
                      rdfs:range :Laboratory ;
                      rdfs:comment "isMemberOfLaboratory is a subproperty of isMember and relates the members of a Laboratory (that can be Researchers or Technologists) to their Laboratory."@en ;
                      rdfs:label "is member of laboratory"@en .


###  http://www.semanticweb.org/italian-research-organization#isMemberOfResearchGroup
:isMemberOfResearchGroup rdf:type owl:ObjectProperty ;
                         rdfs:subPropertyOf :isMemberOf ;
                         rdf:type owl:FunctionalProperty ;
                         rdfs:domain [ rdf:type owl:Class ;
                                       owl:unionOf ( :Researcher
                                                     :Technologist
                                                   )
                                     ] ;
                         rdfs:range :ResearchGroup ;
                         rdfs:comment "isMemberOfResearchGroup is a subproperty of isMember and relates the members of a ReserachGroup (that can be Researchers or Technologists) to their ResearchGroup."@en ;
                         rdfs:label "is member of research group"@en .


###  http://www.semanticweb.org/italian-research-organization#isOfficeOf
:isOfficeOf rdf:type owl:ObjectProperty ;
            rdfs:subPropertyOf :isPartOf ;
            rdf:type owl:FunctionalProperty ;
            rdfs:domain :Office ;
            rdfs:range :Building ;
            rdfs:comment "isOfficeOf is a subproperty of isPartOf and relates offices to the building they belong to"@en ;
            rdfs:label "is office of"@en .


###  http://www.semanticweb.org/italian-research-organization#isPartOf
:isPartOf rdf:type owl:ObjectProperty ,
                   owl:TransitiveProperty ,
                   owl:ReflexiveProperty ;
          rdfs:comment "isPartOf is a superproperty of: isBuildingOf, isInstituteOf, isLaboratoryOf, isMeetingRoomOf, isOfficeOf ans isResearchGroupOf"@en ;
          rdfs:label "is part of"@en .


###  http://www.semanticweb.org/italian-research-organization#isResearchGroupOf
:isResearchGroupOf rdf:type owl:ObjectProperty ;
                   rdfs:subPropertyOf :isPartOf ;
                   rdf:type owl:FunctionalProperty ;
                   rdfs:domain :ResearchGroup ;
                   rdfs:range :Laboratory ;
                   rdfs:comment "isResearchGroupOf is a subproperty of isPartOf and relates research groups to the laboratory of which it is composed"@en ;
                   rdfs:label "is research group of"@en .


###  http://www.semanticweb.org/italian-research-organization#makesContractWith
:makesContractWith rdf:type owl:ObjectProperty ,
                            owl:InverseFunctionalProperty ;
                   rdfs:domain :ResearchOrganisation ;
                   rdfs:range :Employee ;
                   rdfs:comment "makesContracWith relates a research organization to employees that have a contract with it."@en ;
                   rdfs:label "makes contract with"@en .


#################################################################
#    Data properties
#################################################################

###  http://www.semanticweb.org/italian-research-organization#hasEmployeeID
:hasEmployeeID rdf:type owl:DatatypeProperty ;
               rdfs:subPropertyOf :hasID ;
               rdf:type owl:FunctionalProperty ;
               rdfs:domain :Employee ;
               rdfs:range xsd:positiveInteger ;
               owl:propertyDisjointWith :hasOfficeID ;
               rdfs:comment "hasEmployeeID is a subproperty of hasID and relates an employee with his ID that is an integer"^^rdfs:Literal ;
               rdfs:label "has employee ID"^^rdfs:Literal .


###  http://www.semanticweb.org/italian-research-organization#hasID
:hasID rdf:type owl:DatatypeProperty ;
       owl:propertyDisjointWith :hasName ;
       rdfs:comment "hasID is a superproperty of: hasEmployeeID and hasOfficeID"@en ;
       rdfs:label "has ID"^^rdfs:Literal .


###  http://www.semanticweb.org/italian-research-organization#hasInstituteName
:hasInstituteName rdf:type owl:DatatypeProperty ;
                  rdfs:subPropertyOf :hasName ;
                  rdf:type owl:FunctionalProperty ;
                  rdfs:domain :Institute ;
                  rdfs:range xsd:string ;
                  owl:propertyDisjointWith :hasLaboratoryName ,
                                           :hasResearchGroupName ;
                  rdfs:comment "hasIntituteName is a subproperty of hasName and relates an institute to its name that is a string"^^rdfs:Literal ;
                  rdfs:label "has institute name"^^rdfs:Literal .


###  http://www.semanticweb.org/italian-research-organization#hasLaboratoryName
:hasLaboratoryName rdf:type owl:DatatypeProperty ;
                   rdfs:subPropertyOf :hasName ;
                   rdf:type owl:FunctionalProperty ;
                   rdfs:domain :Laboratory ;
                   rdfs:range xsd:string ;
                   owl:propertyDisjointWith :hasResearchGroupName ;
                   rdfs:comment "hasLaboratoryName is a subproperty of hasName and relates a laboratory to its name that is a string"^^rdfs:Literal ;
                   rdfs:label "has laboratory name"^^rdfs:Literal .


###  http://www.semanticweb.org/italian-research-organization#hasName
:hasName rdf:type owl:DatatypeProperty ;
         rdfs:comment "hasName is a superproperty of: hasInstituteName, hasLaboratoryName and hasResearchGroupName"@en ;
         rdfs:label "has name"^^rdfs:Literal .


###  http://www.semanticweb.org/italian-research-organization#hasOfficeID
:hasOfficeID rdf:type owl:DatatypeProperty ;
             rdfs:subPropertyOf :hasID ;
             rdf:type owl:FunctionalProperty ;
             rdfs:domain :Office ;
             rdfs:range xsd:string ;
             rdfs:comment "hasOfficeID is a subproperty of hasID and relates an office to its ID that is a string"^^rdfs:Literal ;
             rdfs:label "has office ID"^^rdfs:Literal .


###  http://www.semanticweb.org/italian-research-organization#hasResearchGroupName
:hasResearchGroupName rdf:type owl:DatatypeProperty ;
                      rdfs:subPropertyOf :hasName ;
                      rdf:type owl:FunctionalProperty ;
                      rdfs:domain :ResearchGroup ;
                      rdfs:range xsd:string ;
                      rdfs:comment "hasResearchGroupName is a subproperty of hasName and relates a research group to its name that is a string"^^rdfs:Literal ;
                      rdfs:label "has research group name"^^rdfs:Literal .


#################################################################
#    Classes
#################################################################

###  http://www.semanticweb.org/italian-research-organization#Building
:Building rdf:type owl:Class ;
          rdfs:subClassOf [ rdf:type owl:Restriction ;
                            owl:onProperty :hasOffice ;
                            owl:someValuesFrom :Office
                          ] ,
                          [ rdf:type owl:Restriction ;
                            owl:onProperty :hasLocation ;
                            owl:qualifiedCardinality "1"^^xsd:nonNegativeInteger ;
                            owl:onClass :Location
                          ] ,
                          [ rdf:type owl:Restriction ;
                            owl:onProperty :hasMeetingRoom ;
                            owl:maxQualifiedCardinality "1"^^xsd:nonNegativeInteger ;
                            owl:onClass :MeetingRoom
                          ] ;
          owl:disjointWith :Employee ,
                           :Institute ,
                           :Laboratory ,
                           :Location ,
                           :Office ,
                           :ResearchGroup ,
                           :ResearchOrganisation ;
          rdfs:comment "A Building is a structure, an edifice that has a location, some offices and can have a meeting room"@en ;
          rdfs:label "building"@en .


###  http://www.semanticweb.org/italian-research-organization#Director
:Director rdf:type owl:Class ;
          rdfs:subClassOf :Researcher ;
          owl:disjointWith :SeniorResearcher ,
                           :YoungResearcher ;
          rdfs:comment "A Director is a person that is an Employee and a Researcher."@en ;
          rdfs:label "director"@en .


###  http://www.semanticweb.org/italian-research-organization#Employee
:Employee rdf:type owl:Class ;
          rdfs:subClassOf :Person ,
                          [ rdf:type owl:Restriction ;
                            owl:onProperty :hasContractWith ;
                            owl:qualifiedCardinality "1"^^xsd:nonNegativeInteger ;
                            owl:onClass :ResearchOrganisation
                          ] ,
                          [ rdf:type owl:Restriction ;
                            owl:onProperty :isHostedIn ;
                            owl:qualifiedCardinality "1"^^xsd:nonNegativeInteger ;
                            owl:onClass :Office
                          ] ,
                          [ rdf:type owl:Restriction ;
                            owl:onProperty :isMemberOf ;
                            owl:qualifiedCardinality "1"^^xsd:nonNegativeInteger ;
                            owl:onClass :Institute
                          ] ,
                          [ rdf:type owl:Restriction ;
                            owl:onProperty :hasEmployeeID ;
                            owl:allValuesFrom xsd:positiveInteger
                          ] ,
                          [ rdf:type owl:Restriction ;
                            owl:onProperty :hasEmployeeID ;
                            owl:qualifiedCardinality "1"^^xsd:nonNegativeInteger ;
                            owl:onDataRange xsd:positiveInteger
                          ] ;
          owl:disjointWith :Institute ,
                           :Laboratory ,
                           :Location ,
                           :Office ,
                           :ResearchGroup ,
                           :ResearchOrganisation ;
          rdfs:comment "An Employee is a person who has a contract with the research organization, has an ID and has an office. An Employee is member of one institute and can be a researcher, a technologist or an office worker."@en ;
          rdfs:label "employee"@en .


###  http://www.semanticweb.org/italian-research-organization#Institute
:Institute rdf:type owl:Class ;
           rdfs:subClassOf [ rdf:type owl:Restriction ;
                             owl:onProperty :hasBuilding ;
                             owl:someValuesFrom :Building
                           ] ,
                           [ rdf:type owl:Restriction ;
                             owl:onProperty :hasLaboratory ;
                             owl:someValuesFrom :Laboratory
                           ] ,
                           [ rdf:type owl:Restriction ;
                             owl:onProperty :hasInstituteName ;
                             owl:qualifiedCardinality "1"^^xsd:nonNegativeInteger ;
                             owl:onDataRange xsd:string
                           ] ;
           owl:disjointWith :Laboratory ,
                            :Location ,
                            :Office ,
                            :ResearchGroup ,
                            :ResearchOrganisation ;
           rdfs:comment "An Institute is part of a research organization. Each Institute has a name, has buildings and consists of more than one laboratory."@en ;
           rdfs:label "institute"@en .


###  http://www.semanticweb.org/italian-research-organization#Laboratory
:Laboratory rdf:type owl:Class ;
            rdfs:subClassOf [ rdf:type owl:Restriction ;
                              owl:onProperty :hasResearchGroup ;
                              owl:minQualifiedCardinality "1"^^xsd:nonNegativeInteger ;
                              owl:onClass :ResearchGroup
                            ] ,
                            [ rdf:type owl:Restriction ;
                              owl:onProperty :hasLaboratoryName ;
                              owl:qualifiedCardinality "1"^^xsd:nonNegativeInteger ;
                              owl:onDataRange xsd:string
                            ] ;
            owl:disjointWith :Location ,
                             :Office ,
                             :ResearchGroup ,
                             :ResearchOrganisation ;
            rdfs:comment "A Laboratory is part of a research organization. Each Laboratory has a name and at least one research group"@en ;
            rdfs:label "laboratory"@en .


###  http://www.semanticweb.org/italian-research-organization#Location
:Location rdf:type owl:Class ;
          owl:disjointWith :Office ,
                           :ResearchGroup ,
                           :ResearchOrganisation ;
          rdfs:comment "A Location is a spatial region or named place."@en ;
          rdfs:label "location"@en .


###  http://www.semanticweb.org/italian-research-organization#MeetingRoom
:MeetingRoom rdf:type owl:Class ;
             rdfs:subClassOf :Room ;
             rdfs:comment "A MeetingRoom is a Room that can be in a Building"@en ;
             rdfs:label "meeting room"@en .


###  http://www.semanticweb.org/italian-research-organization#Office
:Office rdf:type owl:Class ;
        rdfs:subClassOf :Room ,
                        [ rdf:type owl:Restriction ;
                          owl:onProperty :hosts ;
                          owl:someValuesFrom :Employee
                        ] ,
                        [ rdf:type owl:Restriction ;
                          owl:onProperty :hosts ;
                          owl:minQualifiedCardinality "1"^^xsd:nonNegativeInteger ;
                          owl:onClass :Employee
                        ] ,
                        [ rdf:type owl:Restriction ;
                          owl:onProperty :hasOfficeID ;
                          owl:qualifiedCardinality "1"^^xsd:nonNegativeInteger ;
                          owl:onDataRange xsd:string
                        ] ;
        owl:disjointWith :ResearchGroup ,
                         :ResearchOrganisation ;
        rdfs:comment "An Office is a Room that has an ID and hosts one or more employees"@en ;
        rdfs:label "office"@en .


###  http://www.semanticweb.org/italian-research-organization#OfficeWorker
:OfficeWorker rdf:type owl:Class ;
              rdfs:subClassOf :Employee ;
              owl:disjointWith :Researcher ,
                               :Technologist ;
              rdfs:comment "An OfficeWorker is a person and an employee"@en ;
              rdfs:label "office worker"@en .


###  http://www.semanticweb.org/italian-research-organization#Person
:Person rdf:type owl:Class ;
        rdfs:comment "A person can be: office worker,  technologist, (young or senior) researcher,  director, employee."@en ;
        rdfs:label "person"@en .


###  http://www.semanticweb.org/italian-research-organization#ResearchGroup
:ResearchGroup rdf:type owl:Class ;
               rdfs:subClassOf [ rdf:type owl:Restriction ;
                                 owl:onProperty :hasResearchGroupName ;
                                 owl:qualifiedCardinality "1"^^xsd:nonNegativeInteger ;
                                 owl:onDataRange xsd:string
                               ] ;
               owl:disjointWith :ResearchOrganisation ;
               rdfs:comment "A ResearchGroup has a name and is part of a research organization."@en ;
               rdfs:label "research group"@en .


###  http://www.semanticweb.org/italian-research-organization#ResearchOrganisation
:ResearchOrganisation rdf:type owl:Class ;
                      rdfs:subClassOf [ rdf:type owl:Restriction ;
                                        owl:onProperty :hasInstitute ;
                                        owl:someValuesFrom :Institute
                                      ] ;
                      rdfs:comment "A ResearchOrganization makes contracts with employees and consists of more than one institute."@en ;
                      rdfs:label "research organization"@en .


###  http://www.semanticweb.org/italian-research-organization#Researcher
:Researcher rdf:type owl:Class ;
            rdfs:subClassOf :Employee ,
                            [ rdf:type owl:Restriction ;
                              owl:onProperty :isMemberOfLaboratory ;
                              owl:qualifiedCardinality "1"^^xsd:nonNegativeInteger ;
                              owl:onClass :Laboratory
                            ] ,
                            [ rdf:type owl:Restriction ;
                              owl:onProperty :isMemberOfResearchGroup ;
                              owl:qualifiedCardinality "1"^^xsd:nonNegativeInteger ;
                              owl:onClass :ResearchGroup
                            ] ;
            owl:disjointWith :Technologist ;
            rdfs:comment "A Researcher is person that is an employee and can be a YoungResearcher, a SeniorResearcher or a Director. A Researcher is member of one Laboratory and one ResearchGroup."@en ;
            rdfs:label "researcher"@en .


###  http://www.semanticweb.org/italian-research-organization#Room
:Room rdf:type owl:Class ;
      rdfs:comment "A Room can be an Office or a MeetingRoom"@en ;
      rdfs:label "room"@en .


###  http://www.semanticweb.org/italian-research-organization#SeniorResearcher
:SeniorResearcher rdf:type owl:Class ;
                  rdfs:subClassOf :Researcher ;
                  owl:disjointWith :YoungResearcher ;
                  rdfs:comment "A SeniorReseracher is a person that is a Researcher and is senior, so older and more experienced than the other researchers"@en ;
                  rdfs:label "senior researcher"@en .


###  http://www.semanticweb.org/italian-research-organization#Technologist
:Technologist rdf:type owl:Class ;
              rdfs:subClassOf :Employee ,
                              [ rdf:type owl:Restriction ;
                                owl:onProperty :isMemberOfLaboratory ;
                                owl:qualifiedCardinality "1"^^xsd:nonNegativeInteger ;
                                owl:onClass :Laboratory
                              ] ,
                              [ rdf:type owl:Restriction ;
                                owl:onProperty :isMemberOfResearchGroup ;
                                owl:qualifiedCardinality "1"^^xsd:nonNegativeInteger ;
                                owl:onClass :ResearchGroup
                              ] ;
              rdfs:comment "A Technologist is a person and an Employee and is member of one Laboratory and one ResearchGroup."@en ;
              rdfs:label "technologist"@en .


###  http://www.semanticweb.org/italian-research-organization#YoungResearcher
:YoungResearcher rdf:type owl:Class ;
                 rdfs:subClassOf :Researcher ;
                 rdfs:comment "A YoungReseracher is a person that is a Researcher and is young, so at an early stage of research arctivity"@en ;
                 rdfs:label "young researcher"@en .


#################################################################
#    Individuals
#################################################################

###  http://www.semanticweb.org/italian-research-organization#A-03
:A-03 rdf:type owl:NamedIndividual ,
               :Office ;
      :hosts :marioDeFelice ;
      :isOfficeOf :edificio19 ;
      :hasOfficeID "A03"^^xsd:string .


###  http://www.semanticweb.org/italian-research-organization#A-16
:A-16 rdf:type owl:NamedIndividual ,
               :Office ;
      :hosts :marioBerardone ;
      :isOfficeOf :edificio19 ;
      :hasOfficeID "A16"^^xsd:string .


###  http://www.semanticweb.org/italian-research-organization#B-65
:B-65 rdf:type owl:NamedIndividual ,
               :Office ;
      :hosts :andreaMarchetti ;
      :isOfficeOf :edificioB ;
      :hasOfficeID "B65"^^xsd:string .


###  http://www.semanticweb.org/italian-research-organization#C-35
:C-35 rdf:type owl:NamedIndividual ,
               :Office ;
      :hosts :raffaelePerego ;
      :isOfficeOf :edificioB ;
      :hasOfficeID "C35"^^xsd:string .


###  http://www.semanticweb.org/italian-research-organization#CNR
:CNR rdf:type owl:NamedIndividual ,
              :ResearchOrganisation ;
     :hasInstitute :IEOS ,
                   :ISTI ;
     rdfs:label "Consiglio Nazionale delle Ricerche"@it ,
                "National Research Council"@en .


###  http://www.semanticweb.org/italian-research-organization#E-09
:E-09 rdf:type owl:NamedIndividual ,
               :Office ;
      :hosts :sabrinaBattista ;
      :isOfficeOf :edificio19 ;
      :hasOfficeID "E09"^^xsd:string .


###  http://www.semanticweb.org/italian-research-organization#H-13
:H-13 rdf:type owl:NamedIndividual ,
               :Office ;
      :isOfficeOf :edificioA ;
      :hasOfficeID "H13"^^xsd:string .


###  http://www.semanticweb.org/italian-research-organization#HPC
:HPC rdf:type owl:NamedIndividual ,
              :Laboratory ;
     :isLaboratoryOf :ISTI ;
     :hasLaboratoryName "High Performance Computing Laboratory"^^xsd:string .


###  http://www.semanticweb.org/italian-research-organization#I-01
:I-01 rdf:type owl:NamedIndividual ,
               :Office ;
      :hosts :robertoScopigno ;
      :isOfficeOf :edificioB ;
      :hasOfficeID "I01"^^xsd:string .


###  http://www.semanticweb.org/italian-research-organization#I-04
:I-04 rdf:type owl:NamedIndividual ,
               :Office ;
      :hosts :manuelaFerrante ;
      :isOfficeOf :edificioB ;
      :hasOfficeID "I04"^^xsd:string .


###  http://www.semanticweb.org/italian-research-organization#I-11
:I-11 rdf:type owl:NamedIndividual ,
               :Office ;
      :hosts :marcoPuntoni ;
      :isOfficeOf :edificioB ;
      :hasOfficeID "I11"^^xsd:string .


###  http://www.semanticweb.org/italian-research-organization#I-80
:I-80 rdf:type owl:NamedIndividual ,
               :Office ;
      :hosts :claudiaCaudai ;
      :isOfficeOf :edificioB ;
      :hasOfficeID "I80"^^xsd:string .


###  http://www.semanticweb.org/italian-research-organization#IEOS
:IEOS rdf:type owl:NamedIndividual ,
               :Institute ;
      :isInstituteOf :CNR ;
      :hasInstituteName "Istituto per l'endocrinologia e l'oncologia"^^xsd:string .


###  http://www.semanticweb.org/italian-research-organization#IIT
:IIT rdf:type owl:NamedIndividual ,
              :Institute ;
     :isInstituteOf :CNR ;
     :hasInstituteName "Istituto di Informatica e Telematica"^^xsd:string .


###  http://www.semanticweb.org/italian-research-organization#ISTI
:ISTI rdf:type owl:NamedIndividual ,
               :Institute ;
      :isInstituteOf :CNR ;
      :hasInstituteName "Istituto di Scienza e Tecnologie dellâ€™Informazione"^^xsd:string .


###  http://www.semanticweb.org/italian-research-organization#SI
:SI rdf:type owl:NamedIndividual ,
             :Laboratory ;
    :isLaboratoryOf :ISTI ;
    :hasLaboratoryName "Signals and Images"^^xsd:string .


###  http://www.semanticweb.org/italian-research-organization#UI
:UI rdf:type owl:NamedIndividual ,
             :Laboratory ;
    :isLaboratoryOf :IIT ;
    :hasLaboratoryName "Ubiquitous Internet"^^xsd:string .


###  http://www.semanticweb.org/italian-research-organization#andreaMarchetti
:andreaMarchetti rdf:type owl:NamedIndividual ,
                          :Technologist ;
                 :hasContractWith :CNR ;
                 :isMemberOfInstitute :IIT ;
                 :isMemberOfLaboratory :UI ;
                 :isMemberOfResearchGroup :groupUI ;
                 :hasEmployeeID "15392"^^xsd:positiveInteger .


###  http://www.semanticweb.org/italian-research-organization#angelaCeletti
:angelaCeletti rdf:type owl:NamedIndividual ,
                        :SeniorResearcher ;
               :hasContractWith :CNR ;
               :isMemberOfInstitute :IEOS ;
               :hasEmployeeID "18402"^^xsd:positiveInteger .


###  http://www.semanticweb.org/italian-research-organization#angelicaLoDuca
:angelicaLoDuca rdf:type owl:NamedIndividual ,
                         :YoungResearcher ;
                :hasContractWith :CNR ;
                :isHostedIn :B-65 ;
                :isMemberOfInstitute :IIT ;
                :isMemberOfLaboratory :UI ;
                :isMemberOfResearchGroup :groupUI ;
                :hasEmployeeID "13934"^^xsd:positiveInteger .


###  http://www.semanticweb.org/italian-research-organization#aula40
:aula40 rdf:type owl:NamedIndividual ,
                 :MeetingRoom ;
        :isMeetingRoomOf :edificioA .


###  http://www.semanticweb.org/italian-research-organization#aulaSerafinoZappacosta
:aulaSerafinoZappacosta rdf:type owl:NamedIndividual ,
                                 :MeetingRoom ;
                        :isMeetingRoomOf :edificio19 .


###  http://www.semanticweb.org/italian-research-organization#chiaraFalchi
:chiaraFalchi rdf:type owl:NamedIndividual ,
                       :OfficeWorker ;
              :hasContractWith :CNR ;
              :isMemberOfInstitute :ISTI ;
              :hasEmployeeID "15035"^^xsd:positiveInteger .


###  http://www.semanticweb.org/italian-research-organization#claudiaCaudai
:claudiaCaudai rdf:type owl:NamedIndividual ,
                        :YoungResearcher ;
               :hasContractWith :CNR ;
               :isMemberOfInstitute :ISTI ;
               :isMemberOfLaboratory :SI ;
               :isMemberOfResearchGroup :groupSSP ;
               :hasEmployeeID "17355"^^xsd:positiveInteger .


###  http://www.semanticweb.org/italian-research-organization#edificio19
:edificio19 rdf:type owl:NamedIndividual ,
                     :Building ;
            :hasLocation :napoli ;
            :isBuildingOf :IEOS .


###  http://www.semanticweb.org/italian-research-organization#edificioA
:edificioA rdf:type owl:NamedIndividual ,
                    :Building ;
           :hasLocation :pisa ;
           :isBuildingOf :ISTI .


###  http://www.semanticweb.org/italian-research-organization#edificioB
:edificioB rdf:type owl:NamedIndividual ,
                    :Building ;
           :hasLocation :pisa ;
           :isBuildingOf :ISTI .


###  http://www.semanticweb.org/italian-research-organization#gennaroRomano
:gennaroRomano rdf:type owl:NamedIndividual ,
                        :OfficeWorker ;
               :hasContractWith :CNR ;
               :isMemberOfInstitute :IEOS ;
               :hasEmployeeID "19539"^^xsd:positiveInteger .


###  http://www.semanticweb.org/italian-research-organization#giuseppeFusco
:giuseppeFusco rdf:type owl:NamedIndividual ,
                        :Technologist ;
               :hasContractWith :CNR ;
               :isHostedIn :I-04 ;
               :isMemberOfInstitute :ISTI ;
               :isMemberOfLaboratory :SI ;
               :isMemberOfResearchGroup :groupSSP ;
               :hasEmployeeID "16677"^^xsd:positiveInteger .


###  http://www.semanticweb.org/italian-research-organization#groupCB
:groupCB rdf:type owl:NamedIndividual ,
                  :ResearchGroup ;
         :isResearchGroupOf :SI ;
         :hasResearchGroupName "Computational Biology Research Group"^^xsd:string .


###  http://www.semanticweb.org/italian-research-organization#groupHPC
:groupHPC rdf:type owl:NamedIndividual ,
                   :ResearchGroup ;
          :isResearchGroupOf :HPC ;
          :hasResearchGroupName "High Performance Computing Research Group"^^xsd:string .


###  http://www.semanticweb.org/italian-research-organization#groupSSP
:groupSSP rdf:type owl:NamedIndividual ,
                   :ResearchGroup ;
          :isResearchGroupOf :SI ;
          :hasResearchGroupName "Statistical Signal Processing Research Group"^^xsd:string .


###  http://www.semanticweb.org/italian-research-organization#groupUI
:groupUI rdf:type owl:NamedIndividual ,
                  :ResearchGroup ;
         :isResearchGroupOf :UI ;
         :hasResearchGroupName "Ubiquitous Internet Research Group"^^xsd:string .


###  http://www.semanticweb.org/italian-research-organization#immunologia
:immunologia rdf:type owl:NamedIndividual ,
                      :Laboratory ;
             :isLaboratoryOf :IEOS ;
             :hasLaboratoryName "Laboratorio di immunologia"^^xsd:string .


###  http://www.semanticweb.org/italian-research-organization#lidiaBaraldi
:lidiaBaraldi rdf:type owl:NamedIndividual ,
                       :Technologist ;
              :hasContractWith :CNR ;
              :isMemberOfInstitute :IEOS ;
              :hasEmployeeID "12643"^^xsd:positiveInteger .


###  http://www.semanticweb.org/italian-research-organization#lucaCiampi
:lucaCiampi rdf:type owl:NamedIndividual ,
                     :YoungResearcher ;
            :hasContractWith :CNR ;
            :isHostedIn :I-11 ;
            :isMemberOfInstitute :ISTI ;
            :hasEmployeeID "12887"^^xsd:positiveInteger .


###  http://www.semanticweb.org/italian-research-organization#manuelaFerrante
:manuelaFerrante rdf:type owl:NamedIndividual ,
                          :OfficeWorker ;
                 :hasContractWith :CNR ;
                 :isMemberOfInstitute :ISTI ;
                 :hasEmployeeID "17345"^^xsd:positiveInteger .


###  http://www.semanticweb.org/italian-research-organization#marcoPuntoni
:marcoPuntoni rdf:type owl:NamedIndividual ,
                       :Technologist ;
              :hasContractWith :CNR ;
              :isMemberOfInstitute :ISTI ;
              :hasEmployeeID "15246"^^xsd:positiveInteger .


###  http://www.semanticweb.org/italian-research-organization#mariaBucci
:mariaBucci rdf:type owl:NamedIndividual ,
                     :Technologist ;
            :hasContractWith :CNR ;
            :isHostedIn :B-65 ;
            :isMemberOfInstitute :IIT ;
            :isMemberOfLaboratory :UI ;
            :isMemberOfResearchGroup :groupUI ;
            :hasEmployeeID "12666"^^xsd:positiveInteger .


###  http://www.semanticweb.org/italian-research-organization#marioBerardone
:marioBerardone rdf:type owl:NamedIndividual ,
                         :Technologist ;
                :hasContractWith :CNR ;
                :isMemberOfInstitute :IEOS ;
                :hasEmployeeID "19234"^^xsd:positiveInteger .


###  http://www.semanticweb.org/italian-research-organization#marioDeFelice
:marioDeFelice rdf:type owl:NamedIndividual ,
                        :Director ;
               :hasContractWith :CNR ;
               :isMemberOfInstitute :IEOS ;
               :hasEmployeeID "16234"^^xsd:positiveInteger .


###  http://www.semanticweb.org/italian-research-organization#napoli
:napoli rdf:type owl:NamedIndividual ,
                 :Location ;
        :isLocationOf :edificio19 .


###  http://www.semanticweb.org/italian-research-organization#nicolaMessina
:nicolaMessina rdf:type owl:NamedIndividual ,
                        :YoungResearcher ;
               :hasContractWith :CNR ;
               :isHostedIn :I-04 ;
               :isMemberOfInstitute :ISTI ;
               :isMemberOfLaboratory :SI ;
               :hasEmployeeID "14223"^^xsd:positiveInteger .


###  http://www.semanticweb.org/italian-research-organization#pisa
:pisa rdf:type owl:NamedIndividual ,
               :Location ;
      :isLocationOf :edificioB .


###  http://www.semanticweb.org/italian-research-organization#raffaelePerego
:raffaelePerego rdf:type owl:NamedIndividual ,
                         :SeniorResearcher ;
                :hasContractWith :CNR ;
                :isMemberOfInstitute :ISTI ;
                :hasEmployeeID "14987"^^xsd:positiveInteger .


###  http://www.semanticweb.org/italian-research-organization#robertoScopigno
:robertoScopigno rdf:type owl:NamedIndividual ,
                          :Director ;
                 :hasContractWith :CNR ;
                 :isMemberOfInstitute :ISTI ;
                 :hasEmployeeID "17056"^^xsd:positiveInteger .


###  http://www.semanticweb.org/italian-research-organization#sabrinaBattista
:sabrinaBattista rdf:type owl:NamedIndividual ,
                          :YoungResearcher ;
                 :hasContractWith :CNR ;
                 :isMemberOfInstitute :IEOS ;
                 :hasEmployeeID "17162"^^xsd:positiveInteger .


###  http://www.semanticweb.org/italian-research-organization#saraColantonio
:saraColantonio rdf:type owl:NamedIndividual ,
                         :YoungResearcher ;
                :hasContractWith :CNR ;
                :isHostedIn :I-80 ;
                :isMemberOfInstitute :ISTI ;
                :isMemberOfLaboratory :SI ;
                :isMemberOfResearchGroup :groupSSP ;
                :hasEmployeeID "13344"^^xsd:positiveInteger .


###  Generated by the OWL API (version 4.5.9.2019-02-01T07:24:44Z) https://github.com/owlcs/owlapi
